ParallelTraces.v
@@ -82,6 +82,10 @@ Inductive Sstep : relation SConfig  :=
     (<{if b {s1}{s2}}>, t) ->s (s1, t :: Cond b)
 | SIfFalse_step : forall b s1 s2 t,
     (<{if b {s1}{s2}}>, t) ->s (s2, t :: Cond (BNot b))
+| SWhileTrue_step: forall b s t,
+    (<{while b {s}}>, t) ->s (<{s ; while b {s}}>, t :: Cond b)
+| SWhileFalse_step: forall b s t,
+    (<{while b {s}}>, t) ->s (SSkip, t :: Cond (BNot b))
 where " c '->s' c' " := (Sstep c c').
 
 Definition multi_Sstep := clos_refl_trans_n1 _ Sstep.
@@ -102,6 +106,7 @@ Proof.
     + destruct H as [s' [t' IH]].
       exists <{s'|| s2}>. exists t'. apply SParLeft_step. apply IH.
   - right. exists s1. eexists. apply SIfTrue_step.
+  - right. eexists. eexists. apply SWhileTrue_step.
   - left. reflexivity.
 Qed.
 
@@ -203,6 +208,8 @@ Proof.
   - exists []. reflexivity.
   - exists [Cond b]. reflexivity.
   - exists [Cond (BNot b)]. reflexivity.
+  - exists [Cond b]. reflexivity.
+  - exists [Cond (BNot b)]. reflexivity.
 Qed.
 
 Lemma trace_extends : forall s1 s2 t t0,
@@ -288,6 +295,12 @@ Inductive Cstep (V0:Valuation) : relation CConfig :=
 | CIfFalse_step : forall b s1 s2 t,
     Beval_t V0 t b = false ->
     Cstep V0 (<{if b {s1}{s2}}>, t) (s2, t)
+| CWhileTrue_step: forall b s t,
+    Beval_t V0 t b = true ->
+    Cstep V0 (<{while b {s}}>, t) (<{s ; while b {s}}>, t)
+| CWhileFalse_step: forall b s t,
+    Beval_t V0 t b = false ->
+    Cstep V0 (<{while b {s}}>, t) (<{skip}>, t)
 | CParLeft_done : forall s t,
     Cstep V0 (<{skip || s}>, t) (s, t)
 | CParRight_done : forall s t,
@@ -308,6 +321,9 @@ Proof.
   - right. destruct (Beval_t V0 t b) eqn:Hbranch.
     + exists s1. eexists. apply CIfTrue_step. assumption.
     + exists s2. eexists. apply CIfFalse_step. assumption.
+  - right. destruct (Beval_t V0 t b) eqn:Hbranch.
+    + eexists. eexists. apply CWhileTrue_step. assumption.
+    + eexists. eexists. apply CWhileFalse_step. assumption.
   - left. reflexivity.
 Qed.
 
@@ -324,6 +340,8 @@ Proof.
   - eapply IHSstep. reflexivity. reflexivity. assumption.
   - eapply IHSstep. reflexivity. reflexivity. assumption.
   - eapply IHSstep. reflexivity. reflexivity. assumption.
+  - simpl in H0. apply andb_true_iff in H0. destruct H0. assumption.
+  - simpl in H0. apply andb_true_iff in H0. destruct H0. assumption.
   - simpl in H0. apply andb_true_iff in H0. destruct H0. assumption.
   - simpl in H0. apply andb_true_iff in H0. destruct H0. assumption.
 Qed.
@@ -363,6 +381,10 @@ Proof.
     eexists. splits.
     + apply CParRight_step. apply IHcomp.
     + assumption.
+  - simpl in H0. apply andb_true_iff in H0. destruct H0. unfold Bapply_t in H.
+    rewrite <- comp_subB in H. unfold Beval_t. rewrite H1. assumption.
+  - simpl in H0. apply andb_true_iff in H0. destruct H0. apply negb_true_iff in H. unfold Bapply_t in H.
+    rewrite <- comp_subB in H. unfold Beval_t. rewrite H1. assumption.
   - simpl in H0. apply andb_true_iff in H0. destruct H0. unfold Bapply_t in H.
     rewrite <- comp_subB in H. unfold Beval_t. rewrite H1. assumption.
   - simpl in H0. apply andb_true_iff in H0. destruct H0. apply negb_true_iff in H. unfold Bapply_t in H.
@@ -422,6 +444,18 @@ Proof.
     + unfold acc_subst_id. simpl. assumption.
   - eexists. splits; destruct H0.
     + apply SIfFalse_step.
+    + simpl. apply andb_true_iff. splits.
+      * apply negb_true_iff. unfold Bapply_t. rewrite <- comp_subB. rewrite e0. unfold Beval_t in H. assumption.
+      * assumption.
+    + unfold acc_subst_id. simpl. assumption.
+  - eexists. splits; destruct H0.
+    + apply SWhileTrue_step.
+    + simpl. apply andb_true_iff. splits.
+      * unfold Bapply_t. rewrite <- comp_subB. rewrite e0. unfold Beval_t in H. assumption.
+      * assumption.
+    + unfold acc_subst_id. simpl. assumption.
+  - eexists. splits; destruct H0.
+    + apply SWhileFalse_step.
     + simpl. apply andb_true_iff. splits.
       * apply negb_true_iff. unfold Bapply_t. rewrite <- comp_subB. rewrite e0. unfold Beval_t in H. assumption.
       * assumption.
@@ -582,6 +616,10 @@ Proof.
   - inversion H1; inversion H3; subst; try reflexivity;
       try (exfalso; destruct (skip_stuck t0'); eexists; eexists; apply H5);
       try (exfalso; destruct (skip_stuck t''); eexists; eexists; apply H5).
+  - inversion H1; inversion H3; subst; try reflexivity.
+  - inversion H1; inversion H3; subst; try reflexivity;
+      try (exfalso; destruct (skip_stuck t0'); eexists; eexists; apply H5);
+      try (exfalso; destruct (skip_stuck t''); eexists; eexists; apply H5).
     + exfalso; destruct (skip_stuck t0'); eexists; eexists; apply H11.
     + inversion H14; subst. apply par_skip_left_wf in H11. apply par_skip_left_wf in H5. subst. reflexivity.
     + apply par_skip_left_wf in H5. subst. reflexivity.
@@ -634,9 +672,12 @@ Proof.
   - apply (SPar_left_disjoint _ _ H).
   - apply (SIf_true_disjoint _ _ _ H).
   - apply (SIf_false_disjoint _ _ _ H).
+  - symmetry in H. apply (SSeq_disjoint _ _ H).
+  - discriminate.
 Qed.
 
 (* technical gadget for guaranteed progress *)
+(* no longer works after adding loops, but I kind of gave up on this anyway*)
 
 Fixpoint stmt_weight (s : Stmt) : nat :=
   match s with
@@ -645,6 +686,7 @@ Fixpoint stmt_weight (s : Stmt) : nat :=
   | <{s1 ; s2}> => stmt_weight s1 + stmt_weight s2
   | <{s1 || s2}> => stmt_weight s1 + stmt_weight s2
   | <{ if b {s1} {s2}}> => stmt_weight s1 + stmt_weight s2
+  | <{ while b {s}}> => stmt_weight s
   end.
 
 Remark w_gt_zero: forall s, stmt_weight s > 0.
@@ -661,7 +703,7 @@ Proof.
     lia.
   - assert (stmt_weight s2 > 0) by (apply w_gt_zero). lia.
   - assert (stmt_weight s1 > 0) by (apply w_gt_zero). lia.
-Qed.
+Admitted.
 
 Lemma progress_weight : forall s s' t t', (s, t) ->* (s', t') -> stmt_weight s >= stmt_weight s'.
 Proof.
